%% LyX 2.3.6.2 created this file.  For more info, see http://www.lyx.org/.
%% Do not edit unless you really know what you are doing.
\documentclass[english]{article}
\usepackage[latin9]{inputenc}
\usepackage{geometry}
\geometry{verbose,tmargin=2cm,bmargin=2cm,lmargin=2cm,rmargin=2cm,headheight=2cm,headsep=2cm}
\usepackage{amstext}
\usepackage{esint}
\PassOptionsToPackage{normalem}{ulem}
\usepackage{ulem}
\usepackage{babel}
\begin{document}
\title{Aradillas-Lopez Kernel Density Estimation}
\maketitle

\section{Revised Estimation Formula using KDE}

Previously, we implemented the AL bounds as follows:
\[
\frac{1}{T}\sum_{i=1}^{T}max\{r,b_{n-1:n}^{i}\}-v_{0}-G_{n:n}(r)(r-v_{0})\leq\pi_{n}(r)\leq\frac{1}{T}\sum_{i=1}^{T}max\{r,b_{n:n}^{i}\}-v_{0}-\phi_{n-1:n}\left(G_{n:n}(r)\right)^{n}(r-v_{0})
\]
where $T$ is the total number of auctions in the sample, and $b_{n-1:n}^{i}$
is the $2^{nd}$ highest bid in the $i^{th}$ auction in the data.\\
\\
However, this estimation method produces AL bounds that are not very
smooth. To do some smoothing, we re-implement the estimation using
a Kernel Density Estimator, with
\[
\hat{g}_{n-1:n}(v)=\frac{1}{Th}\sum_{i=1}^{T}\mathcal{K}\left(\frac{v-b_{n-1:n}^{i}}{h}\right)
\]
\[
\hat{g}_{n:n}(v)=\frac{1}{Th}\sum_{i=1}^{T}\mathcal{K}\left(\frac{v-b_{n:n}^{i}}{h}\right)
\]
where $T$ is the total number of auctions in the sample, $h$ is
the smoothing parameter for a chosen kernel $\mathcal{K}$, and $b_{n-1:n}^{i}$,
$b_{n:n}^{i}$ are the second highest bid and the highest bid in the
$i^{th}$ auction respectively. \\
\\
Furthermore, set the CDF, 
\[
G_{n:n}(r)=\int_{0}^{r}\hat{g}_{n:n}(v)dv
\]
Then plug these in the equation to create the estimator, 
\[
\int_{0}^{\infty}\text{max}\{r,v\}\hat{g}_{n-1:n}(v)dv-v_{0}-G_{n:n}(r)(r-v_{0})\leq\pi_{n}(r)\leq\int_{0}^{\infty}\text{max}\{r,v\}\hat{g}_{n:n}(v)dv-v_{0}-\phi_{n-1:n}\left(G_{n:n}(r)\right)^{n}(r-v_{0})
\]
I select the Gaussian kernel, with smoothing parameter determined
by the Improved Sheather-Jones (ISJ) method.\\
\\
\\
\textbf{\uline{Lemma}}: $\pi_{L}$ and $\pi_{U}$ are both continous.\\
\\
\[
F_{n:n}(v)\leq\bar{F}_{n:n}(v)\equiv\sum_{m=n+1}^{\bar{n}}\frac{n}{(m-1)m}F_{m-1:m}(v)+\frac{n}{\bar{n}}F_{\bar{n}-1:\bar{n}}(v)
\]
\[
F_{n:n}(v)\geq\text{\ensuremath{\underbar{F}}}_{n:n}(v)\equiv\sum_{m=n+1}^{\bar{n}}\frac{n}{(m-1)m}F_{m-1:m}(v)+\frac{n}{\bar{n}}\left(\phi_{\bar{n}}\left(F_{\bar{n}-1:\bar{n}}(v)\right)\right)^{\bar{n}}
\]
\\
\\
 
\end{document}
